\documentclass[12pt]{article}
\usepackage[utf8]{inputenc}

\title{assn2.2}
\author{
  Daniel Loi\\
  \texttt{dtloi@ucsc.edu}
  \texttt{1547401}
  \and
  Kevin Arellano\\
  \texttt{kcarella@ucsc.edu}
  \texttt{1550271}
  \and
  Claudio Sangeroki\\
  \texttt{csangero@ucsc.edu}
  \texttt{1677403}
}
\date{October 2019}

\begin{document}

\maketitle

\begin{enumerate}
    \item 
    \[P(X_{i} = x_{ij} | Y = y_k) = P(<X_1, X_2, ..., X_n> | Y = y_k) \]
    \[= P(X_1 | Y = y_k) * P(X_2 | Y = y_k) *...*P(X_n | Y = y_k) \]
    \[=\prod_{i=1}^{n}P(X_n | Y = y_k)\]
    \[=\prod_{i=1}^{n}\frac{1}{\sigma\sqrt{2\pi}}exp{\frac{-(x_{i}-\mu)^{2}}{2\sigma^{2}}}\]
    \[=\prod_{i=1}^{n}(\frac{1}{\sigma\sqrt{2\pi}})\prod_{i=1}^{n}(exp{\frac{-(x_{i}-\mu)^{2}}{2\sigma^{2}}})\]
    \[=(\frac{1}{\sigma\sqrt{2\pi}})^n\prod_{i=1}^{n}(exp{\frac{-(x_{i}-\mu)^{2}}{2\sigma^{2}}})\]
    \[=(\frac{1}{\sigma\sqrt{2\pi}})^n(exp\sum_{i=1}^{n}{\frac{-(x_{i}-\mu)^{2}}{2\sigma^{2}}})\]
    \[L(P(X_n | Y = y_k))=log((\frac{1}{\sigma\sqrt{2\pi}})^n(exp\sum_{i=1}^{n}{\frac{-(x_{i}-\mu)^{2}}{2\sigma^{2}}}))\]
    \[=(nlog(\frac{1}{\sigma\sqrt{2\pi}})log(exp\sum_{i=1}^{n}{\frac{-(x_{i}-\mu)^{2}}{2\sigma^{2}}}))\]
    \[=(n(log(1)-log(\sigma\sqrt{2\pi}))log(exp\sum_{i=1}^{n}{\frac{-(x_{i}-\mu)^{2}}{2\sigma^{2}}}))\]
    \[=(n(-log(\sigma)+log(\sqrt{2\pi})))log(exp\sum_{i=1}^{n}{\frac{-(x_{i}-\mu)^{2}}{2\sigma^{2}}}))\]
    \[=(-log(\sigma)n+log(\sqrt{2\pi})n)log(exp\sum_{i=1}^{n}{\frac{-(x_{i}-\mu)^{2}}{2\sigma^{2}}}))\]
    \[=(-log(\sigma)n+log(\sqrt{2\pi})n)(\sum_{i=1}^{n}{\frac{-(x_{i}-\mu)^{2}}{2\sigma^{2}}}))\]
    \[\frac{dL(P(X_n | Y = y_k))}{d\mu}=(-log(\sigma)n+log(\sqrt{2\pi})n)(\sum_{i=1}^{n}{\frac{-(x_{i}-\mu)^{2}}{2\sigma^{2}}}))=0\]
    \[=\sum_{i=1}^{n}{\frac{2((x_{i}-\mu))}{2\sigma^{2}}}=0\]
    \[=\sum_{i=1}^{n}{\frac{(x_{i}-\mu)}{\sigma^{2}}}=0\]
    
    
    
\end{enumerate}
    
\end{document}
